examples/crypto/cryptobox/Box.DH.fst
@@ -42,18 +42,32 @@ assume val hash: dh_element -> Tot aes_key
   Setting up a global log for AE.keys indexed by the ids of the public and private key involved.
 *)
 private type range = fun (k_id:id{AE_id? k_id}) -> k:PlainDH.key{PlainDH.ae_key_get_index k = k_id}
-private let inv (f:MM.map' (i:id{AE_id? i}) range) = True
 
-assume val ae_key_log_region: (r:HH.rid{ extends r root /\ is_eternal_region r /\ is_below r root})
+(**
+   Invariant for the ae_key_log: If a key is honest and we idealize prf_odh, then if it is unfresh,
+   there has to be an entry in the ae_key_log.
+*)
+private let inv (m:MM.map' (i:id{AE_id? i}) range) =
+  forall (i:id{AE_id? i}). (honest i /\ prf_odh) ==> (unfresh i <==> Some? (MM.sel m i))
+  //forall (i:id{AE_id? i}). honest i /\ prf_odh ==> (fresh i h <==> ~(Some? (MM.sel m i)))
+
+
+assume val ae_key_log_region: (r:HH.rid{ extends r root 
+					 /\ is_eternal_region r 
+					 /\ is_below r root 
+					 /\ disjoint r ae_key_region
+					 /\ disjoint r id_freshness_table_region
+					 /\ disjoint r id_honesty_table_region
+					 })
 //private let ae_key_log_region = new_region root
 assume val ae_key_log: MM.t ae_key_log_region (i:id{AE_id? i}) range inv
 //private let ae_key_log = MM.alloc #ae_key_log_region #ae_id #range #inv
 
 noeq abstract type dh_pkey = 
-  | DH_pkey:  #pk_id:id{DH_id? pk_id} -> rawpk:dh_share -> dh_pkey
+  | DH_pkey: #pk_id:id{DH_id? pk_id /\ unfresh pk_id /\ fixed pk_id} -> rawpk:dh_share -> dh_pkey
 
 noeq abstract type dh_skey =
-  | DH_skey: #sk_id:id{DH_id? sk_id} -> rawsk:dh_exponent -> pk:dh_pkey{pk.pk_id=sk_id} -> dh_skey 
+  | DH_skey: #sk_id:id{DH_id? sk_id /\ unfresh sk_id /\ fixed sk_id} -> rawsk:dh_exponent -> pk:dh_pkey{pk.pk_id=sk_id} -> dh_skey 
 
 val sk_get_index: sk:dh_skey -> Tot (i:id{i = sk.sk_id})
 let sk_get_index k = k.sk_id
@@ -74,22 +88,36 @@ val keygen: #i:id{DH_id? i} -> ST (dh_pair:(k:dh_pkey{k.pk_id=i}) * (k:dh_skey{k
   ))
   (ensures (fun h0 k h1 -> 
     unfresh i
-    /\ fixed i
   ))
 let keygen #i =
+  make_unfresh i;
   let dh_share,dh_exponent = dh_gen_key() in
   let dh_pk = DH_pkey #i dh_share in
   let dh_sk = DH_skey #i dh_exponent dh_pk in
-  make_unfresh i;
-  //make_honest i;
   dh_pk,dh_sk
 
-val coerce_pkey: #i:id{DH_id? i /\ dishonest i} -> dh_share -> St (pk:dh_pkey{pk.pk_id=i})
+val coerce_pkey: #i:id{DH_id? i /\ dishonest i} -> dh_share -> ST (pk:dh_pkey{pk.pk_id=i})
+  (requires (fun h0 -> 
+    fresh i h0
+    /\ fixed i
+  ))
+  (ensures (fun h0 pk h1 -> 
+    unfresh i
+  ))
 let coerce_pkey #i dh_sh =
+  make_unfresh i;
   DH_pkey #i dh_sh
 
-val coerce_keypair: #i:id{DH_id? i /\ dishonest i} -> dh_exponent -> St (dh_pair:(k:dh_pkey{k.pk_id=i}) * (k:dh_skey{k.sk_id=i}))
+val coerce_keypair: #i:id{DH_id? i /\ dishonest i} -> dh_exponent -> ST (dh_pair:(k:dh_pkey{k.pk_id=i}) * (k:dh_skey{k.sk_id=i}))
+  (requires (fun h0 -> 
+    fresh i h0
+    /\ fixed i
+  ))
+  (ensures (fun h0 pk h1 -> 
+    unfresh i
+  ))
 let coerce_keypair #i dh_ex =
+  make_unfresh i;
   let dh_sh = dh_exponentiate dh_base dh_ex in
   let pk = DH_pkey #i dh_sh in
   let sk = DH_skey #i dh_ex pk in
@@ -107,68 +135,55 @@ let prf_odhT dh_sk dh_pk =
   k
   
 
-
-//let s:Set.set (r:HH.rid) = Set.union (Set.singleton ae_key_log_region) (Set.singleton ae_key_region)
-
-(**
-   If we prf_odh is true, the output of this function is random, if both 
-   share and exponent are honest.
-*)
 val prf_odh: sk:dh_skey -> pk:dh_pkey -> ST (PlainDH.key)
   ( requires (fun h0 ->
     let i = generate_ae_id pk.pk_id sk.sk_id in
     fixed i
-    /\ (honest i \/ dishonest i)
   ))
   ( ensures (fun h0 k h1 ->
     let i = generate_ae_id pk.pk_id sk.sk_id in
     let s:Set.set (r:HH.rid) = Set.union (Set.singleton ae_key_log_region) (Set.singleton (leak_regionGT k)) in
+    let k_log = leak_logGT k in
     (PlainDH.ae_key_get_index k = i)
-    /\ (honest i \/ dishonest i)
     /\ (
         ( (honest i /\ prf_odh)
-    	    ==> (modifies s h0 h1
-    	       /\ MR.witnessed (MM.contains ae_key_log i k) 
+    	    ==> (//modifies_none h0 h1
+    	       h0 == h1 /\ MR.witnessed (MM.contains ae_key_log i k) 
     	      )
         )
         \/ 
     	( (dishonest i \/ ~prf_odh)
-    	    ==> (modifies_one (PlainDH.leak_regionGT k) h0 h1
-    	       /\ leak_key k = prf_odhT sk pk
+    	    ==> (//modifies_one (PlainDH.leak_regionGT k) h0 h1
+    	       True /\ leak_key k = prf_odhT sk pk
     	      )
         )
       )
+    /\ MR.m_contains k_log h1
   ))
-
-// Proposal: Move the ae_key_log to Box.AE and have AE.keygen guarantee that they output unique keys per ID.
-// Prf-odh can then branch on the prf_odh flag and the honesty of the ae_id to decide if it wants to use keygen
-// or coerce_key. This could break consistency with the formal model. Reduction needed?
-// Prove memory-safety for prf_odh
 let prf_odh dh_sk dh_pk =
-  let pk_id = dh_pk.pk_id in
-  let sk_id = dh_sk.sk_id in
-  let i = generate_ae_id pk_id sk_id in
+  let i = generate_ae_id dh_pk.pk_id dh_sk.sk_id in
   let honest_i = honestST i in
-  if honest_i && prf_odh then
-    (MR.m_recall ae_key_log;
-    let entry = MM.lookup ae_key_log i in
-    match entry with
-    | Some  k' -> k'
-    | None -> 
-      let k' = PlainDH.keygen i in
-      // For some reason, extend violates modifies ... maybe separate regions better?
-      MM.extend ae_key_log i k';
-      k')
+  MR.m_recall ae_key_log;
+  if honest_i && prf_odh then (
+    let h0 = ST.get() in
+    MR.m_recall ae_key_log;
+    match MM.lookup ae_key_log i with
+    | Some  k' ->
+	recall_log k'; 
+        k'
+    | None ->
+	assert(honest i /\ prf_odh);
+        //freshST i;
+	let h = ST.get() in
+	assume(fresh i h);
+        let k' = PlainDH.keygen i in
+	assert(False);
+        MM.extend ae_key_log i k';
+	let h1 = ST.get() in
+        k')
   else(
     assert(dishonest i \/ ~prf_odh);
     let raw_k = dh_exponentiate dh_pk.rawpk dh_sk.rawsk in
     let hashed_raw_k = hash raw_k in
-    assume(disjoint ae_key_region ae_key_log_region);
-    let h0 = ST.get() in
     let k=PlainDH.coerce_key i hashed_raw_k in
-    let h1 = ST.get() in
-    //assert(let s' = Set.singleton (leak_regionGT k) in let s:Set.set (r:HH.rid) = Set.union (Set.singleton ae_key_region) s' in modifies_just s h0.h h1.h);
-//    assert(let s' = Set.singleton (leak_regionGT k) in
-//    let s:Set.set (r:HH.rid) = Set.union (Set.singleton ae_key_region) (Set.singleton s') in modifies s h0 h1);
-    admit();
     k)
