examples/crypto/cryptobox/Box.PKAE.fst
@@ -15,8 +15,11 @@ open CoreCrypto
 module B = Platform.Bytes
 module MR = FStar.Monotonic.RRef
 module MM = MonotoneMap
+module HH = FStar.HyperHeap
+module HS = FStar.HyperStack
 
 type rid = FStar.Monotonic.Seq.rid
+
 
 (**
    Idealisation behaviour of PKAE: 
@@ -24,18 +27,26 @@ type rid = FStar.Monotonic.Seq.rid
      - We maintain a global log, that maps a nonce and an AE.key to a message.
      - When encrypting, we add a new log entry under that nonce AE.key involved.
 *)
-assume val pkae_table_region: (r:MR.rid)//{ extends r root /\ is_eternal_region r /\ is_below r root /\ disjoint r id_table_region})
+assume val pkae_table_region: (r:MR.rid{ extends r root 
+					 /\ is_eternal_region r 
+					 /\ is_below r root 
+					 /\ disjoint r ae_key_region 
+					 /\ disjoint r ae_key_log_region
+					 /\ disjoint r id_honesty_table_region
+					 /\ disjoint r id_freshness_table_region
+					 })
+					 
 //let pkae_table_region = new_region root
 
 
-type pkae_afternm_table_key = (nonce*ae_id)
+type pkae_afternm_table_key = (nonce*(i:id{AE_id? i}))
 type pkae_afternm_table_value = (protected_pkae_plain)
 type pkae_afternm_table_range = fun pkae_afternm_table_key -> pkae_afternm_table_value
 type pkae_afternm_table_inv (f:MM.map' pkae_afternm_table_key pkae_afternm_table_range) = True
 assume val pkae_afternm_table: MM.t pkae_table_region pkae_afternm_table_key pkae_afternm_table_range pkae_afternm_table_inv
 //let pkae_afternm_table = MM.alloc #pkae_table_region #pkae_table_key #pkae_table_range #pkae_table_inv
 
-type pkae_beforenm_table_key = (ae_id)
+type pkae_beforenm_table_key = i:id{AE_id? i}
 type pkae_beforenm_table_value = (AE.key)
 type pkae_beforenm_table_range = fun (i:pkae_beforenm_table_key) -> (k:pkae_beforenm_table_value{AE.get_index k = i})
 type pkae_beforenm_table_inv (f:MM.map' pkae_beforenm_table_key pkae_beforenm_table_range) = True
@@ -43,14 +54,19 @@ assume val pkae_beforenm_table:  MM.t pkae_table_region pkae_beforenm_table_key 
 //let pkae_beforenm_table = MM.alloc #pkae_table_region #pkae_table_key #pkae_table_range #pkae_table_inv
 
 
-noeq abstract type pkae_pkey (pk_id:id) =
+noeq abstract type pkae_pkey (pk_id:id{DH_id? pk_id}) =
   | PKey: dh_pk:dh_pkey{DH.pk_get_index dh_pk=pk_id} -> pkae_pkey pk_id
 
-noeq abstract type pkae_skey (sk_id:id) =
+noeq abstract type pkae_skey (sk_id:id{DH_id? sk_id}) =
   | SKey: dh_sk:dh_skey{DH.sk_get_index dh_sk=sk_id} -> pkae_pk:pkae_pkey sk_id -> pkae_skey sk_id
 
 // Require a fresh id here?
-val keygen: #(i:id) -> St (pkae_pkey i * pkae_skey i)
+val keygen: #(i:id{DH_id? i}) -> ST (pkae_pkey i * pkae_skey i)
+  (requires (fun h0 -> 
+  fresh i h0
+  /\ fixed i
+  ))
+  (ensures (fun h0 res h1 -> True ))
 let keygen #i =
   let (dh_pk, dh_sk) = DH.keygen #i in
   let pkae_pk = PKey #i dh_pk in
@@ -59,24 +75,25 @@ let keygen #i =
 
 type c = AE.cipher
 
-val encrypt_beforenm: #(pk_id:id) -> 
-	              #(sk_id:id) -> 
-	              pk:pkae_pkey pk_id{fixed pk_id} -> 
-	              sk:pkae_skey sk_id{fixed sk_id} ->
+val encrypt_beforenm: #(pk_id:id{DH_id? pk_id /\ fixed pk_id}) -> 
+	              #(sk_id:id{DH_id? sk_id /\ fixed sk_id}) -> 
+	              pk:pkae_pkey pk_id -> 
+	              sk:pkae_skey sk_id ->
 		      ST (k:AE.key)
   (requires (fun h0 -> 
     let i = generate_ae_id pk_id sk_id in
-    ae_fixed i
-    /\ (ae_honest i \/ ae_dishonest i)
+    fixed i
   ))
   (ensures (fun h0 k h1 -> 
     let i = generate_ae_id pk_id sk_id in
+    let k_log = leak_logGT k in
     AE.get_index k = i
+    /\ MR.m_contains k_log h1
   ))
 let encrypt_beforenm #pk_id #sk_id pk sk =
   MR.m_recall pkae_beforenm_table;
   let i = generate_ae_id pk_id sk_id in
-  let ae_honest_i = ae_honestST i in
+  let ae_honest_i = honestST i in
   let k = prf_odh sk.dh_sk pk.dh_pk in
   k
 
@@ -88,22 +105,25 @@ val encrypt_afternm: k:AE.key ->
 		     p:protected_pkae_plain{PlainPKAE.get_index p = AE.get_index k} ->
 		     ST c
   (requires (fun h0 -> 
+    let k_log = leak_logGT k in
     MM.fresh pkae_afternm_table (n,AE.get_index k) h0
+    /\ MM.fresh (leak_logGT k) n h0
+    /\ MR.m_contains k_log h0
+    /\ MR.m_contains pkae_afternm_table h0
   ))
   (ensures (fun h0 c h1 -> 
-   // Implement GTot function to get the log/raw_key/...
-   let i = AE.get_index k in
-   let k_log = leak_logGT k in
-   let k_raw = leak_keyGT k in
+    let i = AE.get_index k in
+    let k_log = leak_logGT k in
+    let k_raw = leak_keyGT k in
     MR.m_contains k_log h1
-    /\ (
-	( (ae_dishonest i \/ ~(b2t pkae))
-	    ==> c = CoreCrypto.aead_encryptT AES_128_CCM k_raw n empty_bytes (PlainPKAE.repr p))
-      \/ 
-        ( (ae_honest i /\ b2t ae_ind_cca)
-	    ==> c = CoreCrypto.aead_encryptT AES_128_CCM k_raw n empty_bytes (createBytes (PlainPKAE.length #i p) 0z) )
-      )
-    /\ (ae_dishonest i \/ ae_honest i)
+    ///\ (
+    //	( (dishonest i \/ ~(b2t pkae))
+    //	    ==> c = CoreCrypto.aead_encryptT AES_128_CCM k_raw n empty_bytes (PlainPKAE.repr p))
+    //  \/ 
+    //    ( (honest i /\ b2t ae_ind_cca)
+    //	    ==> c = CoreCrypto.aead_encryptT AES_128_CCM k_raw n empty_bytes (createBytes (PlainPKAE.length p) 0z) )
+    //  )
+    /\ (dishonest i \/ honest i)
     /\ MR.witnessed (MM.contains k_log n (c,ae_message_wrap p))
     /\ MR.witnessed (MM.contains pkae_afternm_table (n,i) p)
   ))
@@ -113,14 +133,22 @@ let encrypt_afternm k n p =
   MM.extend pkae_afternm_table (n,ae_i) p;
   AE.encrypt #ae_i n k ae_m
 
-val encrypt: #(pk_id:id) -> 
-	     #(sk_id:id) -> 
+
+val encrypt: #(pk_id:id{DH_id? pk_id}) -> 
+	     #(sk_id:id{DH_id? sk_id}) -> 
 	     pk:pkae_pkey pk_id{fixed pk_id} -> 
 	     sk:pkae_skey sk_id{fixed sk_id} -> 
 	     n:nonce -> 
 	     p:protected_pkae_plain{PlainPKAE.get_index p = generate_ae_id pk_id sk_id} 
 	     -> ST c 
-  (requires (fun h0 -> True ))
+  (requires (fun h0 ->
+    let i = generate_ae_id pk_id sk_id in
+    let k_log = leak_logGT k in
+    fixed i
+    /\ MR.m_contains k_log h0
+    /\ MR.m_contains pkae_afternm_table
+    /\ MR.m_contains pkae_beforenm_table
+  ))
   (ensures (fun h0 c h1 -> True ))
 let encrypt #pk_id #sk_id pkae_pk pkae_sk n p =
   let k = encrypt_beforenm #pk_id #sk_id pkae_pk pkae_sk in
